Start incrementalising Move

isabelle/Move.thy
@@ -5,6 +5,11 @@ begin
 datatype 'oid tree_op =
   Assign "'oid" "string" "'oid" "'oid set"
 
+lemma tree_op_assign:
+  assumes "\<And>obj key val prev. x = Assign obj key val prev \<Longrightarrow> P"
+  shows "P"
+using assms tree_op.exhaust by blast
+
 fun tree_op_deps :: "'oid tree_op \<Rightarrow> 'oid set" where
   "tree_op_deps (Assign obj key val prev) = {obj, val} \<union> prev"
 
@@ -38,31 +43,26 @@ fun sorted_oplist :: "('oid::{linorder} \<times> 'oid tree_op) list \<Rightarrow
   "sorted_oplist [] oper = [oper]"
 
 lemma sorted_oplist_insert:
-  shows "\<exists>as bs. xs = as @ bs \<and> sorted_oplist xs oper = as @ [oper] @ bs \<and>
-         (\<forall>a \<in> set as. fst a < fst oper) \<and> (bs \<noteq> [] \<longrightarrow> fst oper \<le> fst (hd bs))"
+  shows "\<exists>as bs. xs = as @ bs \<and> sorted_oplist xs oper = as @ [oper] @ bs"
 proof(induction xs, simp)
   case (Cons x xs)
   obtain i1 op1 where "x = (i1, op1)" by fastforce
   obtain i2 op2 where "oper = (i2, op2)" by fastforce
-  show "\<exists>as bs. x # xs = as @ bs \<and> sorted_oplist (x # xs) oper = as @ [oper] @ bs \<and>
-         (\<forall>a \<in> set as. fst a < fst oper) \<and> (bs \<noteq> [] \<longrightarrow> fst oper \<le> fst (hd bs))"
+  show "\<exists>as bs. x # xs = as @ bs \<and> sorted_oplist (x # xs) oper = as @ [oper] @ bs"
   proof(cases "i1 < i2")
     case True
     moreover from this have "sorted_oplist (x # xs) oper = x # (sorted_oplist xs oper)"
       by (simp add: \<open>oper = (i2, op2)\<close> \<open>x = (i1, op1)\<close>)
-    moreover obtain as bs where "xs = as @ bs \<and> sorted_oplist xs oper = as @ [oper] @ bs \<and>
-         (\<forall>a \<in> set as. fst a < fst oper) \<and> (bs \<noteq> [] \<longrightarrow> fst oper \<le> fst (hd bs))"
+    moreover obtain as bs where "xs = as @ bs \<and> sorted_oplist xs oper = as @ [oper] @ bs"
       using Cons.IH by blast
-    ultimately have "x # xs = (x # as) @ bs \<and> sorted_oplist (x # xs) oper = (x # as) @ [oper] @ bs \<and>
-         (\<forall>a \<in> set (x # as). fst a < fst oper) \<and> (bs \<noteq> [] \<longrightarrow> fst oper \<le> fst (hd bs))"
+    ultimately have "x # xs = (x # as) @ bs \<and> sorted_oplist (x # xs) oper = (x # as) @ [oper] @ bs"
       using \<open>oper = (i2, op2)\<close> \<open>x = (i1, op1)\<close> by auto
     then show ?thesis by blast
   next
     case False
     moreover from this have "sorted_oplist (x # xs) oper = oper # x # xs"
       by (simp add: \<open>oper = (i2, op2)\<close> \<open>x = (i1, op1)\<close>)
-    ultimately have "x # xs = [] @ (x # xs) \<and> sorted_oplist (x # xs) oper = [] @ [oper] @ (x # xs) \<and>
-         (\<forall>a \<in> set []. fst a < fst oper) \<and> (x # xs \<noteq> [] \<longrightarrow> fst oper \<le> fst (hd (x # xs)))"
+    ultimately have "x # xs = [] @ (x # xs) \<and> sorted_oplist (x # xs) oper = [] @ [oper] @ (x # xs)"
       using \<open>oper = (i2, op2)\<close> \<open>x = (i1, op1)\<close> by auto
     then show ?thesis by blast
   qed
@@ -152,5 +152,192 @@ lemma sorted_oplist_commute:
          sorted_oplist (sorted_oplist xs (i2, op2)) (i1, op1)"
 by (metis assms neqE sorted_oplist_commute_base)
 
+
+fun interp_op :: "('oid::{linorder} \<times> 'oid tree_op) list \<times> ('oid \<times> 'oid \<times> string \<times> 'oid) set
+   \<Rightarrow> ('oid \<times> 'oid tree_op) \<Rightarrow> ('oid \<times> 'oid tree_op) list \<times> ('oid \<times> 'oid \<times> string \<times> 'oid) set" where
+  "interp_op (ops, _) oper = (
+      let oplist = sorted_oplist ops oper
+      in (oplist, interp_tree oplist))"
+
+lemma interp_op_commute:
+  assumes "fst op1 \<noteq> fst op2"
+  shows "interp_op (interp_op s op1) op2 = interp_op (interp_op s op2) op1"
+proof -
+  obtain oplist E where "s = (oplist, E)" by fastforce
+  have "fst (interp_op (interp_op s op1) op2) = sorted_oplist (sorted_oplist oplist op1) op2"
+    by (metis \<open>s = (oplist, E)\<close> fst_conv interp_op.simps)
+  moreover have "fst (interp_op (interp_op s op2) op1) = sorted_oplist (sorted_oplist oplist op2) op1"
+    by (metis \<open>s = (oplist, E)\<close> fst_conv interp_op.simps)
+  moreover have "sorted_oplist (sorted_oplist oplist op1) op2 = sorted_oplist (sorted_oplist oplist op2) op1"
+    by (metis assms prod.collapse sorted_oplist_commute)
+  moreover have "snd (interp_op (interp_op s op1) op2) = interp_tree (fst (interp_op (interp_op s op1) op2))"
+    by (metis \<open>s = (oplist, E)\<close> calculation(1) interp_op.simps snd_conv)
+  ultimately show ?thesis
+    by (metis \<open>s = (oplist, E)\<close> interp_op.simps)
+qed
+
+(* list of (oid, oper, flag) triples *)
+
+fun tree_spec' :: "('oid \<times> 'oid \<times> string \<times> 'oid) set \<Rightarrow> ('oid \<times> 'oid tree_op \<times> bool) \<Rightarrow> ('oid \<times> 'oid \<times> string \<times> 'oid) set" where
+  "tree_spec' E (oid, Assign obj key val prev, valid) = (
+     if valid then
+       { e \<in> E. fst e \<notin> prev \<and> snd (snd (snd e)) \<noteq> val } \<union>
+       { (oid, obj, key, val) }
+     else E)"
+
+definition interp_tree' :: "('oid \<times> 'oid tree_op \<times> bool) list \<Rightarrow> ('oid \<times> 'oid \<times> string \<times> 'oid) set" where
+  "interp_tree' ops \<equiv> foldl tree_spec' {} ops"
+
+fun append_op :: "('oid::{linorder} \<times> 'oid tree_op) \<Rightarrow> ('oid \<times> 'oid tree_op \<times> bool) list \<Rightarrow>
+                  ('oid \<times> 'oid tree_op \<times> bool) list" where
+  "append_op (oid, Assign obj key val prev) ops =
+     (let valid = \<not> ancestor (interp_tree' ops) val obj
+      in ops @ [(oid, Assign obj key val prev, valid)])"
+
+fun reapply_ops :: "('oid::{linorder} \<times> 'oid tree_op \<times> bool) list \<Rightarrow> ('oid \<times> 'oid tree_op \<times> bool) list \<Rightarrow>
+                    ('oid \<times> 'oid tree_op \<times> bool) list" where
+  "reapply_ops ((oid, oper, flag) # xs) ops = reapply_ops xs (append_op (oid, oper) ops)" |
+  "reapply_ops [] ops = ops"
+
+fun add_op :: "('oid::{linorder} \<times> 'oid tree_op) \<Rightarrow> ('oid \<times> 'oid tree_op \<times> bool) list \<Rightarrow>
+               ('oid \<times> 'oid tree_op \<times> bool) list \<Rightarrow> ('oid \<times> 'oid tree_op \<times> bool) list" where
+  "add_op newop (x # xs) ops =
+     (if fst x < fst newop
+      then add_op newop xs (ops @ [x])
+      else reapply_ops (x # xs) (append_op newop ops))" |
+  "add_op newop [] ops = append_op newop ops"
+
+definition add_op1 :: "('oid::{linorder} \<times> 'oid tree_op \<times> bool) list \<Rightarrow> ('oid::{linorder} \<times> 'oid tree_op) \<Rightarrow> ('oid \<times> 'oid tree_op \<times> bool) list" where
+  "add_op1 ops newop \<equiv> add_op newop ops []"
+
+lemma add_op_cons:
+  shows "map (\<lambda>x. (fst x, fst (snd x))) (add_op (nid, nop) xs [x]) =
+    (fst x, fst (snd x)) # map (\<lambda>x. (fst x, fst (snd x))) (add_op (nid, nop) xs [])"
+proof(induction xs)
+  case Nil
+  obtain obj key val prev where "nop = Assign obj key val prev"
+    using tree_op.exhaust by blast
+  then show ?case by auto
+next
+  case (Cons a xs)
+  then show ?case sorry
+qed
+
+lemma append_op_map_fst:
+  shows "map fst (append_op (oid, oper) ops) = map fst ops @ [oid]"
+proof -
+  obtain obj key val prev where "oper = Assign obj key val prev"
+    using tree_op.exhaust by blast
+  hence "append_op (oid, oper) ops = ops @ [(oid, oper, \<not> ancestor (interp_tree' ops) val obj)]"
+    by simp
+  thus ?thesis by auto
+qed
+
+lemma reapply_ops_last:
+  shows "reapply_ops (xs @ [x]) ops = append_op (fst x, fst (snd x)) (reapply_ops xs ops)"
+proof(induction xs)
+  case Nil
+  then show ?case
+    by (metis (no_types, lifting) Cons_eq_append_conv prod.collapse reapply_ops.simps(1) reapply_ops.simps(2))
+next
+  case (Cons a xs)
+  hence "reapply_ops ((a # xs) @ [x]) ops =
+         reapply_ops (xs @ [x]) (append_op (fst x, fst (snd x)) ops)"
+    sorry
+  then show ?case sorry
+      
+qed
+
+lemma reapply_ops_map:
+  shows "map fst (reapply_ops xs ops) = map fst (ops @ xs)"
+proof(induction xs rule: List.rev_induct, simp)
+  case (snoc x xs)
+  then show ?case sorry
+qed
+
+lemma reapply_ops_map:
+  shows "map fst (reapply_ops xs ops) = map fst (ops @ xs)"
+proof(induction xs, simp)
+  case (Cons a xs)
+  have "map fst (reapply_ops (a # xs) ops) =
+        map fst (reapply_ops xs (append_op (fst a, fst (snd a)) ops))"
+    by (metis prod.collapse reapply_ops.simps(1))
+  moreover have "append_op (fst a, fst (snd a)) ops = ops @ [(fst a, fst (snd a), \<not> ancestor (interp_tree' ops) val obj)]"
+    sorry
+  then show ?case sorry
+qed
+
+lemma add_op1_result:
+  assumes "ys = map (\<lambda>x. (fst x, fst (snd x))) xs"
+  shows "sorted_oplist ys (nid, nop) = map (\<lambda>x. (fst x, fst (snd x))) (add_op1 xs (nid, nop))"
+using assms proof(induction xs arbitrary: ys)
+  case Nil
+  hence "sorted_oplist ys (nid, nop) = [(nid, nop)]"
+    by simp
+  moreover obtain obj key val prev where "nop = Assign obj key val prev"
+    using tree_op.exhaust by blast
+  hence "add_op1 [] (nid, nop) = [(nid, nop, \<not> ancestor (interp_tree' []) val obj)]"
+    by (simp add: add_op1_def)
+  hence "map (\<lambda>x. (fst x, fst (snd x))) (add_op1 [] (nid, nop)) = [(nid, nop)]"
+    by simp
+  ultimately show ?case by auto
+next
+  case (Cons x xs)
+  obtain xi xo xv where "x = (xi, xo, xv)" by (metis prod.collapse)
+  obtain obj key val prev where "nop = Assign obj key val prev"
+    using tree_op.exhaust by blast
+  show ?case
+  proof(cases "xi < nid")
+    case True
+    then show ?thesis
+      by (simp add: Cons.IH Cons.prems \<open>x = (xi, xo, xv)\<close> add_op1_def add_op_cons)
+  next
+    case False
+    hence "sorted_oplist ys (nid, nop) = [(nid, nop)] @ ys"
+      using Cons.prems \<open>x = (xi, xo, xv)\<close> by auto
+    moreover have "add_op1 (x # xs) (nid, nop) =
+         reapply_ops (x # xs) [(nid, nop, \<not> ancestor (interp_tree' []) val obj)]"
+      by (simp add: \<open>nop = Assign obj key val prev\<close> \<open>x = (xi, xo, xv)\<close> add_op1_def False)
+    then show ?thesis sorry
+  qed
+qed
+
+lemma add_op1_fold:
+  shows "foldl sorted_oplist [] ops = map (\<lambda>x. (fst x, fst (snd x))) (foldl add_op1 [] ops)"
+proof(induction ops rule: List.rev_induct, simp)
+  case (snoc x xs)
+  obtain xid xop where "x = (xid, xop)" by fastforce
+  then show ?case
+    by (simp add: add_op1_result snoc.IH)
+qed
+
+    
+lemma interp_equal:
+  shows "interp_tree (foldl sorted_oplist [] ops) = interp_tree' (foldl add_op1 [] ops)"
+proof(induction ops rule: List.rev_induct)
+  case Nil
+  then show ?case by (simp add: interp_tree'_def interp_tree_def)
+next
+  case (snoc x xs)
+  obtain oid obj key val prev where "x = (oid, Assign obj key val prev)"
+    by (meson prod.simps(1) tree_spec.cases)
+  have "foldl sorted_oplist [] (xs @ [x]) = sorted_oplist (foldl sorted_oplist [] xs) x"
+    by simp
+  have "foldl tree_spec {} (foldl sorted_oplist [] xs) = foldl tree_spec' {} (foldl add_op1 [] xs)"
+    using interp_tree'_def interp_tree_def snoc.IH by blast
+  then show ?case sorry
+qed    
+
+lemma add_op_test:
+  assumes "i1 < i2" and "i2 < i3" and "i3 < i4" and "i4 < i5"
+    and "o3 = Assign j3 k3 v3 p3"
+    and "o4 = Assign j4 k4 v4 p4"
+    and "o5 = Assign j5 k5 v5 p5"
+  shows "add_op (i3, o3) [(i1, o1, v1), (i2, o2, v2), (i4, o4, v4), (i5, o5, v5)] [] =
+         [(i1, o1, v1), (i2, o2, v2), (i3, o3, v3'), (i4, o4, v4'), (i5, o5, v5')] \<and>
+         v3' = (\<not> ancestor (interp_tree' [(i1, o1, v1), (i2, o2, v2)]) v3 j3) \<and>
+         v4' = (\<not> ancestor (interp_tree' [(i1, o1, v1), (i2, o2, v2), (i3, o3, v3')]) v4 j4) \<and>
+         v5' = (\<not> ancestor (interp_tree' [(i1, o1, v1), (i2, o2, v2), (i3, o3, v3'), (i4, o4, v4')]) v5 j5)"
+using assms(2) assms(3) by auto
 
 end
